ODPLL: more

Weidenbach_Book/CDCL_Extensions/DPLL_W_Optimal_Model.thy
@@ -265,6 +265,27 @@ interpretation dpll: dpll\<^sub>W_state trail clauses tl_trail cons_trail state_
   apply (auto simp: state cons_trail dpll.additional_info_def)
   done
 
+inductive backtrack_opt :: \<open>'st \<Rightarrow> 'st \<Rightarrow> bool\<close> where
+backtrack_opt: "backtrack_split (trail S) = (M', L # M) \<Longrightarrow> is_decided L \<Longrightarrow> D \<in># conflicting_clss S
+  \<Longrightarrow> trail S \<Turnstile>as CNot D
+  \<Longrightarrow> state' T = (Propagated (- (lit_of L)) () # M, clauses S, weight S, conflicting_clss S)
+  \<Longrightarrow> backtrack_opt S T"
+
+inductive backtrack :: \<open>'st \<Rightarrow> 'st \<Rightarrow> bool\<close> where
+backtrack: "backtrack_split (trail S) = (M', L # M) \<Longrightarrow> is_decided L \<Longrightarrow> D \<in># clauses S
+  \<Longrightarrow> trail S \<Turnstile>as CNot D
+  \<Longrightarrow> state' T = (Propagated (- (lit_of L)) () # M, clauses S, weight S, conflicting_clss S)
+  \<Longrightarrow> trail S \<Turnstile>as CNot D \<Longrightarrow> backtrack S T"
+
+inductive propagate :: "'st \<Rightarrow> 'st \<Rightarrow> bool" for S T where
+propagate: "add_mset L C \<in># clauses S \<Longrightarrow> trail S \<Turnstile>as CNot C \<Longrightarrow> undefined_lit (trail S) L \<Longrightarrow>
+  T \<sim> cons_trail (Propagated L ()) S \<Longrightarrow>
+  propagate S T"
+
+inductive decide :: "'st \<Rightarrow> 'st \<Rightarrow> bool" for S T where
+decide: "undefined_lit (trail S) L \<Longrightarrow> atm_of L \<in> atms_of_mm (clauses S) \<Longrightarrow>
+  T \<sim> cons_trail (Decided L) S \<Longrightarrow>
+  decide S T"
 
 text \<open>
   In the definition below the \<^term>\<open>state' T = (Propagated L () # trail
@@ -278,20 +299,10 @@ text \<open>
   to the last decision independantly of the conflict.
 \<close>
 inductive dpll\<^sub>W_core :: "'st \<Rightarrow> 'st \<Rightarrow> bool" for S T where
-propagate: "add_mset L C \<in># clauses S \<Longrightarrow> trail S \<Turnstile>as CNot C \<Longrightarrow> undefined_lit (trail S) L \<Longrightarrow>
-  T \<sim> cons_trail (Propagated L ()) S \<Longrightarrow>
-  dpll\<^sub>W_core S T" |
-decided: "undefined_lit (trail S) L \<Longrightarrow> atm_of L \<in> atms_of_mm (clauses S) \<Longrightarrow>
-  T \<sim> cons_trail (Decided L) S \<Longrightarrow>
-  dpll\<^sub>W_core S T " |
-backtrack: "backtrack_split (trail S) = (M', L # M) \<Longrightarrow> is_decided L \<Longrightarrow> D \<in># clauses S
-  \<Longrightarrow> trail S \<Turnstile>as CNot D
-  \<Longrightarrow> state' T = (Propagated (- (lit_of L)) () # M, clauses S, weight S, conflicting_clss S)
-  \<Longrightarrow> trail S \<Turnstile>as CNot D \<Longrightarrow> dpll\<^sub>W_core S T" |
-backtrack_opt: "backtrack_split (trail S) = (M', L # M) \<Longrightarrow> is_decided L \<Longrightarrow> D \<in># conflicting_clss S
-  \<Longrightarrow> trail S \<Turnstile>as CNot D
-  \<Longrightarrow> state' T = (Propagated (- (lit_of L)) () # M, clauses S, weight S, conflicting_clss S)
-  \<Longrightarrow> dpll\<^sub>W_core S T"
+propagate: "propagate S T \<Longrightarrow> dpll\<^sub>W_core S T" |
+decided: "decide S T \<Longrightarrow> dpll\<^sub>W_core S T " |
+backtrack: "backtrack S T \<Longrightarrow> dpll\<^sub>W_core S T" |
+backtrack_opt: \<open>backtrack_opt S T \<Longrightarrow> dpll\<^sub>W_core S T\<close>
 
 inductive_cases dpll\<^sub>W_coreE: \<open>dpll\<^sub>W_core S T\<close>
 
@@ -309,19 +320,19 @@ bnb:
   if \<open>dpll\<^sub>W_branch S T\<close>
 
 inductive_cases dpll\<^sub>W_bnbE: \<open>dpll\<^sub>W_bnb S T\<close>
-
+find_theorems atms_of_mm conflicting_clss
 lemma dpll\<^sub>W_core_is_dpll\<^sub>W:
   \<open>dpll\<^sub>W_core S T \<Longrightarrow> dpll\<^sub>W (abs_state S) (abs_state T)\<close>
   supply abs_state_def[simp] state'_def[simp]
   apply (induction rule: dpll\<^sub>W_core.induct)
   subgoal
-    by (auto simp: dpll\<^sub>W.simps dest!: )
+    by (auto simp: dpll\<^sub>W.simps propagate.simps)
   subgoal
-    by (auto simp: dpll\<^sub>W.simps dest!: )
+    by (auto simp: dpll\<^sub>W.simps decide.simps)
   subgoal
-    by (auto simp: dpll\<^sub>W.simps)
+    by (auto simp: dpll\<^sub>W.simps backtrack.simps)
   subgoal
-    by (auto simp: dpll\<^sub>W.simps)
+    by (auto simp: dpll\<^sub>W.simps backtrack_opt.simps)
   done
 
 lemma dpll\<^sub>W_core_abs_state_all_inv:
@@ -333,13 +344,13 @@ lemma dpll\<^sub>W_core_same_weight:
   supply abs_state_def[simp] state'_def[simp]
   apply (induction rule: dpll\<^sub>W_core.induct)
   subgoal
-    by (auto simp: dpll\<^sub>W.simps)
+    by (auto simp: dpll\<^sub>W.simps propagate.simps)
   subgoal
-    by (auto simp: dpll\<^sub>W.simps)
+    by (auto simp: dpll\<^sub>W.simps decide.simps)
   subgoal
-    by (auto simp: dpll\<^sub>W.simps)
+    by (auto simp: dpll\<^sub>W.simps backtrack.simps)
   subgoal
-    by (auto simp: dpll\<^sub>W.simps)
+    by (auto simp: dpll\<^sub>W.simps backtrack_opt.simps)
   done
 
 lemma dpll\<^sub>W_branch_trail:
@@ -382,13 +393,13 @@ lemma dpll\<^sub>W_core_clauses:
   supply abs_state_def[simp] state'_def[simp]
   apply (induction rule: dpll\<^sub>W_core.induct)
   subgoal
-    by (auto simp: dpll\<^sub>W.simps)
+    by (auto simp: dpll\<^sub>W.simps propagate.simps)
   subgoal
-    by (auto simp: dpll\<^sub>W.simps)
+    by (auto simp: dpll\<^sub>W.simps decide.simps)
   subgoal
-    by (auto simp: dpll\<^sub>W.simps)
+    by (auto simp: dpll\<^sub>W.simps  backtrack.simps)
   subgoal
-    by (auto simp: dpll\<^sub>W.simps)
+    by (auto simp: dpll\<^sub>W.simps  backtrack_opt.simps)
   done
 
 lemma dpll\<^sub>W_bnb_clauses:
@@ -466,19 +477,24 @@ lemma dpll\<^sub>W_core_Ex_propagate:
    Ex (dpll\<^sub>W_core S)"
   subgoal
     by (rule exI[of _ \<open>cons_trail (Propagated L ()) S\<close>])
-     (fastforce simp: dpll\<^sub>W_core.simps state_eq_ref)
+     (fastforce simp: dpll\<^sub>W_core.simps state_eq_ref propagate.simps)
   subgoal
     by (rule exI[of _ \<open>cons_trail (Decided L) S\<close>])
-     (auto simp: dpll\<^sub>W_core.simps state'_def)
+      (auto simp: dpll\<^sub>W_core.simps state'_def decide.simps backtrack.simps backtrack_opt.simps
+        propagate.simps)
   subgoal
     using backtrack_split_list_eq[of \<open>trail S\<close>, symmetric] apply -
     apply (rule exI[of _ \<open>cons_trail (Propagated (-lit_of L') ()) ((tl_trail ^^ (length (L' # M'))) S)\<close>])
-    apply (auto simp: dpll\<^sub>W_core.simps state'_def state_tl_trail_comp_pow funpow_tl_append_skip_ge)
+    apply (auto simp: dpll\<^sub>W_core.simps state'_def state_tl_trail_comp_pow funpow_tl_append_skip_ge
+       decide.simps backtrack.simps backtrack_opt.simps
+        propagate.simps)
     done
   subgoal
     using backtrack_split_list_eq[of \<open>trail S\<close>, symmetric] apply -
     apply (rule exI[of _ \<open>cons_trail (Propagated (-lit_of L') ()) ((tl_trail ^^ (length (L' # M'))) S)\<close>])
-    apply (auto simp: dpll\<^sub>W_core.simps state'_def state_tl_trail_comp_pow funpow_tl_append_skip_ge)
+    apply (auto simp: dpll\<^sub>W_core.simps state'_def state_tl_trail_comp_pow funpow_tl_append_skip_ge
+       decide.simps backtrack.simps backtrack_opt.simps
+        propagate.simps)
     done
   done
 
@@ -497,7 +513,9 @@ proof -
                   defined_lit (trail S) L\<close> for L
     using spec[OF ns, of \<open>cons_trail _ S\<close>]
     apply (fastforce simp: dpll\<^sub>W_bnb.simps total_over_m_def total_over_set_def
-      dpll\<^sub>W_core.simps state'_def)
+      dpll\<^sub>W_core.simps state'_def
+       decide.simps backtrack.simps backtrack_opt.simps
+        propagate.simps)
     done
   have [intro]: \<open>is_decided L \<Longrightarrow>
        backtrack_split (trail S) = (M', L # M) \<Longrightarrow>
@@ -542,7 +560,9 @@ proof (rule ccontr)
   have no_decide: \<open>atm_of L \<in> atms_of_mm (clauses S) \<Longrightarrow> defined_lit (trail S) L\<close> for L
     using spec[OF ns, of \<open>cons_trail _ S\<close>]
     apply (fastforce simp: dpll\<^sub>W_bnb.simps total_over_m_def total_over_set_def
-      dpll\<^sub>W_core.simps state'_def)
+      dpll\<^sub>W_core.simps state'_def 
+       decide.simps backtrack.simps backtrack_opt.simps
+        propagate.simps)
     done
   have tot: \<open>total_over_m (lits_of_l (trail S)) (set_mset (clauses S))\<close>
     using no_decide
@@ -769,7 +789,9 @@ lemma cdcl_bnb_still_model:
   using assms
 proof (induction rule: bnb.dpll\<^sub>W_bnb.induct)
   case (dpll S T)
-  then show ?case using ent by (auto elim!: bnb.dpll\<^sub>W_coreE simp: bnb.state'_def)
+  then show ?case using ent by (auto elim!: bnb.dpll\<^sub>W_coreE simp: bnb.state'_def 
+       bnb.decide.simps bnb.backtrack.simps bnb.backtrack_opt.simps
+       bnb.propagate.simps)
 next
   case (bnb S T)
   then show ?case
