Weidenbach_Book/CDCL_Extensions/DPLL_W_Partial_Encoding.thy
@@ -1,0 +1,50 @@
+theory DPLL_W_Partial_Encoding
+imports
+  DPLL_W_Optimal_Model
+  CDCL_W_Partial_Encoding
+begin
+
+locale dpll_optimal_encoding_opt =
+  dpll\<^sub>W_state_optimal_weight trail clauses
+    tl_trail cons_trail state_eq state   \<rho> update_additional_info +
+  optimal_encoding_opt_ops \<Sigma> \<Delta>\<Sigma> new_vars 
+  for
+    trail :: \<open>'st \<Rightarrow> 'v  dpll\<^sub>W_ann_lits\<close> and
+    clauses :: \<open>'st \<Rightarrow> 'v clauses\<close> and
+    tl_trail :: \<open>'st \<Rightarrow> 'st\<close> and
+    cons_trail :: \<open>'v  dpll\<^sub>W_ann_lit \<Rightarrow> 'st \<Rightarrow> 'st\<close> and
+    state_eq  :: \<open>'st \<Rightarrow> 'st \<Rightarrow> bool\<close> (infix "\<sim>" 50) and
+    state :: \<open>'st \<Rightarrow> 'v  dpll\<^sub>W_ann_lits \<times> 'v clauses \<times> 'v clause option \<times> 'b\<close> and
+    update_additional_info :: \<open>'v clause option \<times> 'b \<Rightarrow> 'st \<Rightarrow> 'st\<close> and
+    \<Sigma> \<Delta>\<Sigma> :: \<open>'v set\<close> and
+    \<rho> :: \<open>'v clause \<Rightarrow> 'a :: {linorder}\<close> and
+    new_vars :: \<open>'v \<Rightarrow> 'v \<times> 'v\<close>
+begin
+
+end
+
+
+locale dpll_optimal_encoding =
+  dpll_optimal_encoding_opt trail clauses
+    tl_trail cons_trail state_eq state
+    update_additional_info \<Sigma> \<Delta>\<Sigma> \<rho> new_vars  +
+  optimal_encoding_ops
+    \<Sigma> \<Delta>\<Sigma>
+    new_vars \<rho>
+  for
+    trail :: \<open>'st \<Rightarrow> 'v  dpll\<^sub>W_ann_lits\<close> and
+    clauses :: \<open>'st \<Rightarrow> 'v clauses\<close> and
+    tl_trail :: \<open>'st \<Rightarrow> 'st\<close> and
+    cons_trail :: \<open>'v  dpll\<^sub>W_ann_lit \<Rightarrow> 'st \<Rightarrow> 'st\<close> and
+    state_eq  :: \<open>'st \<Rightarrow> 'st \<Rightarrow> bool\<close> (infix "\<sim>" 50) and
+    state :: \<open>'st \<Rightarrow> 'v  dpll\<^sub>W_ann_lits \<times> 'v clauses \<times> 'v clause option \<times> 'b\<close> and
+    update_additional_info :: \<open>'v clause option \<times> 'b \<Rightarrow> 'st \<Rightarrow> 'st\<close> and
+    \<Sigma> \<Delta>\<Sigma> :: \<open>'v set\<close> and
+    \<rho> :: \<open>'v clause \<Rightarrow> 'a :: {linorder}\<close> and
+    new_vars :: \<open>'v \<Rightarrow> 'v \<times> 'v\<close>
+begin
+
+
+end
+
+end
